newio/GPDM.fst
@@ -1,0 +1,217 @@
+module GPDM
+
+open FStar.Classical.Sugar
+open FStar.List.Tot.Base
+open FStar.Tactics
+
+
+(** a tentative to generalize Partial Dijkstra Monads **)
+
+(** A Dijkstra monad D A w is a monad-like structure that classifies effectful 
+computations returning values in A and specified by w : W A. **)
+
+(** In DM4ALL, it is shown that a computational monad M A, a specification monad W A, and a monad
+morphism between the two (called theta), give rise to a Dijkstra Monad. **)
+
+assume type m (a:Type)
+assume val return_m : a:Type -> x:a -> m a
+
+(** this is new and needed to define a Partial Dijkstra Monad **)
+assume val is_return_of : #a:Type -> x:a -> m a -> Type0
+assume val lemma_is_return_of_return_m : unit -> Lemma (forall a (x:a). x `is_return_of` return_m _ x)
+
+assume val bind_m : a:Type -> b:Type -> l:(m a) -> k:((x:a{x `is_return_of` l}) -> m b) -> m b
+
+assume val lemma_is_return_of_bind_m : 
+  a:Type -> 
+  b:Type ->
+  l:m a ->
+  lx:a{lx `is_return_of` l} -> 
+  k:(x:a{x `is_return_of` l} -> m b) -> 
+  Lemma (forall kx. kx `is_return_of` (k lx) ==> kx `is_return_of` (bind_m a b l k))
+
+assume type w (a:Type)
+assume val return_w : a:Type -> x:a -> w a
+assume val bind_w : a:Type -> b:Type -> w a -> (a -> w b) -> w b
+
+assume val ord_w : #a:Type -> wp1:w a -> wp2:w a -> Type0
+assume val lemma_ord_w_id : #a:Type -> wp1:w a -> Lemma (wp1 `ord_w` wp1)
+
+(** I think we can implement this, and it should be just the identiy fuction. **)
+assume val subcomp_w : #a:Type -> #p1:(a -> Type0) -> #p2:(a -> Type0) -> wp:w (x:a{p1 x}) -> Pure (w (x:a{p2 x}))
+  (requires (forall x. p1 x ==> p2 x)) 
+  (ensures (fun _ -> True))
+
+assume val lift_pure_pre_to_w : #a:Type -> pure_pre -> w a
+
+assume val lemma_ord_w_lift_pure_pre_to_w : #a:Type -> (x:a) -> Lemma (return_w a x `ord_w` (lift_pure_pre_to_w True))
+  
+assume val theta : a:Type -> (l:m a) -> w (x:a{x `is_return_of` l})
+
+assume val lemma_theta_is_monad_morphism_ret : #a:Type -> x:a ->
+  Lemma (subcomp_w (theta a (return_m a x)) == return_w a x)
+
+assume val lemma_theta_is_monad_morphism_bind :
+  a:Type ->
+  b:Type ->
+  l:m a ->
+  k:(x:a{x `is_return_of` l} -> m b) ->
+  Lemma (theta b (bind_m a b l k) == bind_w (x:a{x `is_return_of` l}) (x:b{x `is_return_of` bind_m a b l k}) (theta a l) (fun x -> 
+    lemma_is_return_of_bind_m a b l x k;
+    subcomp_w (theta b (k x))))
+
+let dm (a:Type) (wp:w a) = l:(m a){wp `ord_w` (subcomp_w (theta a l))}
+
+let return_dm (a:Type) (x:a) : dm a (return_w a x) = 
+  lemma_theta_is_monad_morphism_ret x;
+  lemma_ord_w_id (return_w a x);
+  return_m a x
+
+val bind_dm :
+  a:Type ->
+  b:Type -> 
+  lwp:w a ->
+  kwp:(a -> w b) ->
+  l:dm a lwp ->
+  k:(x:a{x `is_return_of` l} -> dm b (kwp x)) ->
+  dm b (bind_w _ _ lwp kwp)
+let bind_dm a b lwp kwp l k =
+  (** I think this proof should be similar to the one from DM4ALL **)
+  lemma_theta_is_monad_morphism_bind a b l k;
+  (**
+  (** from the lemma: **)
+  assert (theta (bind_m l k) == bind_w _ _ (theta l) (fun x -> lemma_is_return_of_bind_m a b l x k; subcomp_w (theta _ (k x))));
+  (** from the types **)
+  assert (lwp `ord_w` (subcomp_w (theta a l));
+  assert (forall (x:a{x `is_return_of` l}). kwp x `ord_w` (subcomp_w (theta b (k x))));
+
+  assert (bind_w a b lwp kwp `ord_w`
+  	   bind_w (x:a{x `is_return_of` v}) _ (theta l) (fun x -> theta (k x)));
+	   
+  (** goal: **)
+  assert (bind_w _ b lwp kwp `hist_ord #_ #b` theta (bind_m v f));**)
+  admit ();
+  bind_m a b l k
+
+(** A few problems before going forward:
+  1. The `forall p h. wp p h ==> pre` is to specific. There is no `p` and `h`.
+     Maybe trying Guido's idea would be interesting:
+       wp `ord_w` lift_pure_pre_to_w pre
+
+  2. 
+**)
+
+let pdm (a:Type) (wp:w a) = 
+  pre : pure_pre { wp `ord_w` (lift_pure_pre_to_w pre) } & (squash pre -> dm a wp)
+
+let get_pre #a #wp (t : pdm a wp) : Pure pure_pre (requires True) (ensures fun r -> wp `ord_w` (lift_pure_pre_to_w r)) =
+  let (| pre , f |) = t in pre
+
+let get_fun #a #w (t : pdm a w) : Pure (dm a w) (requires get_pre t) (ensures fun _ -> True) =
+  let (| pre, f |) = t in f ()
+
+let pdm_return (a:Type) (x:a) : pdm a (return_w a x) =
+  lemma_ord_w_lift_pure_pre_to_w x;
+ (| True, (fun _ -> return_dm a x) |)
+
+let pdm_bind (a b:Type)
+  (wp1:w a) (wp2:a -> w b)
+  (f:pdm a wp1) 
+  (g:(x:a) -> pdm b (wp2 x)) :
+  pdm b (bind_w a b wp1 wp2) =
+  assert (wp1 `ord_w` (lift_pure_pre_to_w (get_pre f)));
+  assume (lift_pure_pre_to_w (get_pre f) ==> get_pre f);
+  assert (wp1 `ord_w` subcomp_w (theta a (get_fun f)));
+  assert (forall x. x `is_return_of` (get_fun f) ==> wp2 x `ord_w` theta b (get_fun (g x)));
+  assume (bind_w a b wp1 wp2 `ord_w` (lift_pure_pre_to_w (get_pre f /\ (forall x. x `is_return_of` (get_fun f) ==> get_pre (g x)))));
+  (| (get_pre f /\ (forall x. x `is_return_of` (get_fun f) ==> get_pre (g x))), 
+     (fun _ -> 
+       bind_dm a b wp1 wp2 (get_fun f) (fun x -> get_fun (g x))) 
+   |)
+
+let pdm_subcomp (a:Type) (wp1:hist a) (wp2:hist a) (f:pdm a wp1) :
+  Pure (pdm a wp2)
+    (requires (wp2 `hist_ord` wp1))
+    (ensures fun _ -> True) =
+  (| get_pre f, (fun _ -> dm_subcomp a wp1 wp2 (get_fun f)) |)
+
+unfold
+let pdm_if_then_else 
+  (a : Type)
+  (wp1: hist a)
+  (wp2: hist a)
+  (f : pdm a wp1)
+  (g : pdm a wp2)
+  (b : bool) : Type =
+  pdm a (hist_if_then_else wp1 wp2 b)
+
+total
+reifiable
+reflectable
+effect {
+  IOwp (a:Type) (wp : hist #event a) 
+  with {
+       repr       = pdm
+     ; return     = pdm_return
+     ; bind       = pdm_bind 
+     ; subcomp    = pdm_subcomp
+     ; if_then_else = pdm_if_then_else
+     }
+}
+
+effect IO
+  (a:Type)
+  (pre : trace -> Type0)
+  (post : trace -> trace -> a -> Type0) =
+  IOwp a 
+    (fun (p:hist_post a) (h:trace) -> pre h /\ (forall lt r. post h lt r ==>  p lt r)) 
+
+let lift_pure_pdm (a : Type) 
+  (w : pure_wp a)
+  (f:(eqtype_as_type unit -> PURE a w)) : 
+  pdm a (wp_lift_pure_hist w) =
+  lemma_wp_lift_pure_hist_implies_as_requires #a #event w;
+  (| as_requires w, (fun _ -> 
+    FStar.Monotonic.Pure.elim_pure_wp_monotonicity_forall ();
+    let r = f () in
+    let r' = dm_return _ r in
+    dm_subcomp _ _ _ r' ) |)
+
+sub_effect PURE ~> IOwp = lift_pure_pdm
+  
+assume val p : prop
+assume val p' : prop
+assume val pure_lemma (_:unit) : Lemma p
+assume val some_f (_:squash p) : IO unit (fun _ -> True) (fun _ _ _ -> True)
+assume val some_f' : unit -> IO unit (requires (fun _ -> p)) (ensures fun _ _ _ -> p')
+
+let test () : IO unit (fun _ -> True) (fun _ _ _ -> True) =
+  pure_lemma ();
+  some_f ()
+
+let test'' () : IO unit (fun _ -> True) (fun _ _ _ -> True) =
+  pure_lemma ();
+  some_f ();
+  some_f' ();
+  assert p'
+
+let static_cmd
+  (cmd : io_cmds)
+  (argz : io_args cmd) :
+  IO (io_resm cmd)
+    (requires (fun h -> io_pre cmd argz h))
+    (ensures (fun h lt r ->
+        lt == [convert_call_to_event cmd argz r])) =
+  IOwp?.reflect (| True,  (fun _ -> io_call cmd argz) |)
+
+let testStatic3 (fd:file_descr) : IO unit (fun h -> is_open fd h) (fun h lt r -> ~(is_open fd (List.rev lt @ h))) =
+  let _ = static_cmd Close fd in
+  ()
+
+let testStatic2 () : IO unit (fun _ -> True) (fun _ _ _ -> True) =
+  let fd = static_cmd Openfile "../Makefile" in
+  if Some? fd then begin (** test if Openfile was successful **)
+    let msg = static_cmd Read (Some?.v fd) in
+    let _ = static_cmd Close (Some?.v fd) in
+    ()
+  end else ()
